@prefix : <https://w3id.org/iprok/integrated#> .
@prefix owl: <http://www.w3.org/2002/07/owl#> .
@prefix rdfs: <http://www.w3.org/2000/01/rdf-schema#> .
@prefix xsd: <http://www.w3.org/2001/XMLSchema#> .

<https://w3id.org/iprok/integrated> a owl:Ontology ;
    owl:imports <https://w3id.org/iprok>,
        <https://w3id.org/iprok/cost>,
        <https://w3id.org/iprok/resource>,
        <https://w3id.org/iprok/schedule> .

:allocatedUnits a owl:DatatypeProperty,
        owl:FunctionalProperty ;
    rdfs:label "allocated Units"^^xsd:string ;
    rdfs:comment "The specific quantity or number of units of a resource assigned in this allocation (e.g., 40 hours, 5 pieces)."^^xsd:string ;
    rdfs:domain :ResourceAllocation ;
    rdfs:range xsd:decimal .

:allocationActualStartDate a owl:DatatypeProperty,
        owl:FunctionalProperty ;
    rdfs:label "allocation Actual Start Date"^^xsd:string ;
    rdfs:comment "The actual start date and time of this specific resource allocation."^^xsd:string ;
    rdfs:domain :ResourceAllocation ;
    rdfs:range xsd:dateTime .

:allocationAssignsResource a owl:FunctionalProperty,
        owl:ObjectProperty ;
    rdfs:label "allocation Assigns Resource"^^xsd:string ;
    rdfs:comment "Links this resource allocation instance to the specific Resource being assigned."^^xsd:string ;
    rdfs:domain :ResourceAllocation ;
    rdfs:range <https://w3id.org/iprok/resource#Resource> .

:allocationForTask a owl:FunctionalProperty,
        owl:ObjectProperty ;
    rdfs:label "allocation For Task"^^xsd:string ;
    rdfs:comment "Links this resource allocation instance to the specific Task it is assigned to."^^xsd:string ;
    rdfs:domain :ResourceAllocation ;
    rdfs:range <https://w3id.org/iprok/schedule#Task> .

:allocationPlannedFinishDate a owl:DatatypeProperty,
        owl:FunctionalProperty ;
    rdfs:label "allocation Planned Finish Date"^^xsd:string ;
    rdfs:comment "The planned finish date and time for this specific resource allocation."^^xsd:string ;
    rdfs:domain :ResourceAllocation ;
    rdfs:range xsd:dateTime .

:allocationPlannedStartDate a owl:DatatypeProperty,
        owl:FunctionalProperty ;
    rdfs:label "allocation Planned Start Date"^^xsd:string ;
    rdfs:comment "The planned start date and time for this specific resource allocation."^^xsd:string ;
    rdfs:domain :ResourceAllocation ;
    rdfs:range xsd:dateTime .

:resourceAllocationIncursCostItem a owl:ObjectProperty ;
    rdfs:label "resource Allocation Incurs Cost Item"^^xsd:string ;
    rdfs:comment "Links a specific ResourceAllocation to a CostItem that is incurred due to the usage of the allocated resource."^^xsd:string ;
    rdfs:domain :ResourceAllocation ;
    rdfs:range <https://w3id.org/iprok/cost#CostItem> .

:taskGeneratesCostItem a owl:ObjectProperty ;
    rdfs:label "task Generates Cost Item"^^xsd:string ;
    rdfs:comment "Links a Task to a CostItem that is generated or incurred as a result of performing the task."^^xsd:string ;
    rdfs:domain <https://w3id.org/iprok/schedule#Task> ;
    rdfs:range <https://w3id.org/iprok/cost#CostItem> .

:taskHasResourceAllocation a owl:ObjectProperty ;
    rdfs:label "task Has Resource Allocation"^^xsd:string ;
    rdfs:comment "Links a Task to its specific ResourceAllocation instance(s), detailing how resources are assigned to it."^^xsd:string ;
    rdfs:domain <https://w3id.org/iprok/schedule#Task> ;
    rdfs:range :ResourceAllocation .

:ResourceAllocation a owl:Class ;
    rdfs:label "Resource Allocation"^^xsd:string ;
    rdfs:comment "Represents the specific assignment of a quantity of a resource to a task over a defined period, detailing how resources are utilized for work."^^xsd:string ;
    rdfs:subClassOf <https://w3id.org/iprok#IproKThing> .

